more

thys/Generic_Barendregt_Enhanced_Rule_Induction.thy
@@ -102,260 +102,299 @@ lemma small_two[simp,intro!]: "small {x,y}"
 lemma small_three[simp,intro!]: "small {x,y,z}" 
   by (simp add: inf_A small_def)
 
-end (* context Small *)
-
-
-locale Components = Small dummy 
-for dummy :: 'A 
-+
-fixes (* 'T: term-like entities *)
-Tmap :: "('A \<Rightarrow> 'A) \<Rightarrow> 'T \<Rightarrow> 'T"
-and Tfvars :: "'T \<Rightarrow> 'A set"
-assumes  
-Tmap_id: "Tmap id = id"
-and 
-Tmap_comp: "\<And>\<sigma> \<tau>. ssbij \<sigma> \<Longrightarrow> ssbij \<tau> \<Longrightarrow> Tmap (\<sigma> o \<tau>) = Tmap \<sigma> o Tmap \<tau>"
-and 
-small_Tfvars: "\<And>t. small (Tfvars t)" 
-and (* the weaker, inclusion-based version is sufficient (and similarly for V): *)
-Tmap_Tfvars: "\<And>t \<sigma>. ssbij \<sigma> \<Longrightarrow> Tfvars (Tmap \<sigma> t) \<subseteq> \<sigma> ` (Tfvars t)"
-and 
-Tmap_cong_id: "\<And>t \<sigma>. ssbij \<sigma> \<Longrightarrow> (\<forall>a\<in>Tfvars t. \<sigma> a = a) \<Longrightarrow> Tmap \<sigma> t = t"
-begin
-
-lemma Tmap_comp': "\<And>\<sigma> \<tau> t. ssbij \<sigma> \<Longrightarrow> ssbij \<tau> \<Longrightarrow> Tmap (\<sigma> o \<tau>) t = Tmap \<sigma> (Tmap \<tau> t)"
-using Tmap_comp by fastforce 
-
 lemma small_image: "small B \<Longrightarrow> small (\<sigma> ` B)"
 using card_of_image ordLeq_ordLess_trans small_def by blast
 
 lemmas image_comp' = image_comp[symmetric]
 
+end (* context Small *)
+
+
+locale CComponents = Small dummy 
+for dummy :: 'A 
++
+fixes (* 'T: term-like entities, ranged over by t *)
+Tmap :: "('A \<Rightarrow> 'A) \<Rightarrow> 'T \<Rightarrow> 'T"
+and Tfvars :: "'T \<Rightarrow> 'A set"
+      (* 'B: binder-like entities, ranged over by xs *)
+and Bmap :: "('A \<Rightarrow> 'A) \<Rightarrow> 'B \<Rightarrow> 'B"
+and Bvars :: "'B \<Rightarrow> 'A set"
+(* well-formed binders: *)
+and wfB :: "'B \<Rightarrow> bool" 
+assumes  
+Tmap_id[simp]: "Tmap id = id"
+and 
+Tmap_comp: "\<And>\<sigma> \<tau>. ssbij \<sigma> \<Longrightarrow> ssbij \<tau> \<Longrightarrow> Tmap (\<sigma> o \<tau>) = Tmap \<sigma> o Tmap \<tau>"
+and 
+small_Tfvars: "\<And>t. small (Tfvars t)" 
+and (* the weaker, inclusion-based version is sufficient (and similarly for B): *)
+Tmap_Tfvars: "\<And>t \<sigma>. ssbij \<sigma> \<Longrightarrow> Tfvars (Tmap \<sigma> t) \<subseteq> \<sigma> ` (Tfvars t)"
+and 
+Tmap_cong_id: "\<And>t \<sigma>. ssbij \<sigma> \<Longrightarrow> (\<forall>a\<in>Tfvars t. \<sigma> a = a) \<Longrightarrow> Tmap \<sigma> t = t"
+and 
+Bmap_id[simp]: "Bmap id = id"
+and 
+Bmap_comp: "\<And>\<sigma> \<tau>. ssbij \<sigma> \<Longrightarrow> ssbij \<tau> \<Longrightarrow> Bmap (\<sigma> o \<tau>) = Bmap \<sigma> o Bmap \<tau>"
+and 
+small_Bvars: "\<And>xs. wfB xs \<Longrightarrow> small (Bvars xs)" 
+and 
+Bmap_Bvars: "\<And>xs \<sigma>. ssbij \<sigma> \<Longrightarrow> Bvars (Bmap \<sigma> xs) \<subseteq> \<sigma> ` (Bvars xs)"
+and 
+Bmap_cong_id: "\<And>xs \<sigma>. ssbij \<sigma> \<Longrightarrow> (\<forall>a\<in>Bvars xs. \<sigma> a = a) \<Longrightarrow> Bmap \<sigma> xs = xs"
+begin
+
+(* Being smaller than the number of well-formed binders: *)
+definition bsmall :: "'A set \<Rightarrow> bool" where "bsmall X \<equiv> |X| <o |{xs . wfB xs}|"
+
+lemma Tmap_comp': "ssbij \<sigma> \<Longrightarrow> ssbij \<tau> \<Longrightarrow> Tmap (\<sigma> o \<tau>) t = Tmap \<sigma> (Tmap \<tau> t)"
+using Tmap_comp by fastforce 
+
 lemma image_Tfvars_disj: "ssbij \<sigma> \<Longrightarrow> B \<inter> Tfvars t = {} \<Longrightarrow> image \<sigma> B \<inter> Tfvars (Tmap \<sigma> t) = {}"
 using Tmap_Tfvars ssbij_bij by fastforce
 
+lemma Bmap_comp': "ssbij \<sigma> \<Longrightarrow> ssbij \<tau> \<Longrightarrow> Bmap (\<sigma> o \<tau>) xs = Bmap \<sigma> (Bmap \<tau> xs)"
+using Bmap_comp by fastforce 
+
+lemma image_Bvars_disj: "ssbij \<sigma> \<Longrightarrow> B \<inter> Bvars xs = {} \<Longrightarrow> image \<sigma> B \<inter> Bvars (Bmap \<sigma> xs) = {}"
+using Bmap_Bvars ssbij_bij by fastforce
 
 (* *)
 
-end (* locale Components *)
+definition wfBij :: "('A \<Rightarrow> 'A) \<Rightarrow> bool" 
+where "wfBij \<sigma> \<equiv> \<forall>xs. wfB xs \<longleftrightarrow> wfB (Bmap \<sigma> xs)"
+
+
+lemma wfBij_id[simp,intro]: "wfBij id"
+unfolding wfBij_def by auto
+
+lemma wfBij_comp[simp]: 
+"ssbij \<sigma> \<Longrightarrow> wfBij \<sigma> \<Longrightarrow> ssbij \<tau> \<Longrightarrow> wfBij \<tau> \<Longrightarrow> wfBij (\<tau> o \<sigma>)"
+by (simp add: Bmap_comp' wfBij_def)
+
+lemma wfBij_inv[simp]: "ssbij \<sigma> \<Longrightarrow> wfBij \<sigma> \<Longrightarrow> wfBij (inv \<sigma>)"
+by (metis Bmap_comp' Bmap_id id_apply ssbij_inv ssbij_invL wfBij_def)
+
+end (* locale CComponents *)
 
 
 
-(* GENERAL VERSIONS OF THE LOCALES, WITH wfBij AND closed *)
+(* GENERAL VERSIIONS OF THE LOCALES, WIITH wfBij AND closed *)
 
-locale IInduct1 = Components dummy Tmap Tfvars 
+locale IInduct1 = CComponents dummy Tmap Tfvars Bmap Bvars wfB
 for dummy :: 'A 
-and
-Tmap :: "('A \<Rightarrow> 'A) \<Rightarrow> 'T \<Rightarrow> 'T"
+and Tmap :: "('A \<Rightarrow> 'A) \<Rightarrow> 'T \<Rightarrow> 'T"
 and Tfvars :: "'T \<Rightarrow> 'A set"
+and Bmap :: "('A \<Rightarrow> 'A) \<Rightarrow> 'B \<Rightarrow> 'B"
+and Bvars :: "'B \<Rightarrow> 'A set"
+and wfB 
 +
 fixes (* The operator that defines the inductive predicate as lfp:  *)
-G :: "('T \<Rightarrow> bool) \<Rightarrow> 'A set \<Rightarrow> 'T \<Rightarrow> bool"
-and 
-closed :: "'A set \<Rightarrow> bool" 
-and 
-wfBij :: "('A \<Rightarrow> 'A) \<Rightarrow> bool"
+GG :: "('T \<Rightarrow> bool) \<Rightarrow> 'B \<Rightarrow> 'T \<Rightarrow> bool"
+(* *)
 assumes 
-G_mmono: "\<And>R R' B t. R \<le> R' \<Longrightarrow> small B \<Longrightarrow> G R B t \<Longrightarrow> G R' B t"
+GG_mmono: "\<And>R R' xs t. R \<le> R' \<Longrightarrow> GG R xs t \<Longrightarrow> GG R' xs t"
 and 
-G_eequiv: "\<And>\<sigma> R B t. ssbij \<sigma> \<Longrightarrow> wfBij \<sigma> \<Longrightarrow> small B \<Longrightarrow> G R B t \<Longrightarrow> G (\<lambda>t'. R (Tmap (inv \<sigma>) t')) (image \<sigma> B) (Tmap \<sigma> t)"
+GG_eequiv: "\<And>\<sigma> R xs t. ssbij \<sigma> \<Longrightarrow> wfBij \<sigma> \<Longrightarrow> 
+   GG R xs t \<Longrightarrow> GG (\<lambda>t'. R (Tmap (inv \<sigma>) t')) (Bmap \<sigma> xs) (Tmap \<sigma> t)"
 and 
 (* *)
-G_closed: "\<And>R B t. G R B t \<Longrightarrow> closed B"
+GG_wfB: "\<And>R xs t. GG R xs t \<Longrightarrow> wfB xs"
 and 
-wfBij_id[simp,intro]: "wfBij id"
-and 
-wfBij_comp[simp]: "\<And>\<sigma> \<tau>. ssbij \<sigma> \<Longrightarrow> wfBij \<sigma> \<Longrightarrow> ssbij \<tau> \<Longrightarrow> wfBij \<tau> \<Longrightarrow> wfBij (\<tau> o \<sigma>)"
-and 
-wfBij_inv[simp]: "\<And>\<sigma>. ssbij \<sigma> \<Longrightarrow> wfBij \<sigma> \<Longrightarrow> wfBij (inv \<sigma>)"
-and 
-closed_wfBij: "\<And>\<sigma>. ssbij \<sigma> \<Longrightarrow> wfBij \<sigma> \<Longrightarrow> closed A \<Longrightarrow> closed (\<sigma> ` A)"
-and 
-small_ssbij_closed: 
+(* 
+extend_wfBij: 
 "\<And>A A' B. small A \<Longrightarrow> small B \<Longrightarrow> small A' \<Longrightarrow> A \<inter> A' = {} \<Longrightarrow> closed A
-           \<Longrightarrow> \<exists>\<rho>. ssbij \<rho> \<and> wfBij \<rho> \<and> \<rho> ` A \<inter> B = {} \<and> (\<forall>a\<in>A'. \<rho> a = a)"
+           \<Longrightarrow> \<exists>\<rho>. ssbij \<rho> \<and> wfBij \<rho> \<and> \<rho> ` A \<inter> B = {} \<and> (\<forall>a\<in>A'. \<rho> a = a)" *)
+extend_wfBij: 
+"\<And>A. small A \<Longrightarrow> bsmall A \<Longrightarrow> bij_betw \<rho> A B \<Longrightarrow> wfBij \<rho> \<Longrightarrow> 
+     \<exists>\<rho>'. ssbij \<rho>' \<and> wfBij \<rho>' \<and> (\<forall>a\<in>A. \<rho>' a = \<rho> a)"
 begin
 
-lemma G_small_mono[mono]: "\<And>R R' B t.  R \<le> R' \<Longrightarrow> small B \<and> G R B t \<longrightarrow> small B \<and> G R' B t"
-  using G_mmono by blast
+lemma GG_mmono2[mono]: "\<And>R R' xs t.  R \<le> R' \<Longrightarrow> GG R xs t \<longrightarrow> GG R' xs t"
+  using GG_mmono by blast
 
-inductive I :: "'T \<Rightarrow> bool" where 
-G_I_intro: "small B \<Longrightarrow> G I B t \<Longrightarrow> I t"
 
-lemma "I \<equiv> lfp (\<lambda>R t. \<exists>B. small B \<and> G R B t)"
-using I_def[simplified] .
+inductive II :: "'T \<Rightarrow> bool" where 
+GG_II_intro: "GG II xs t \<Longrightarrow> II t"
+
+lemma "II \<equiv> lfp (\<lambda>R t. \<exists>xs. GG R xs t)"
+using II_def[simplified] .
  
-lemma I_equiv: 
-assumes "I t" and \<sigma>: "ssbij \<sigma>" "wfBij \<sigma>"
-shows "I (Tmap \<sigma> t)"
+lemma II_equiv: 
+assumes "II t" and \<sigma>: "ssbij \<sigma>" "wfBij \<sigma>"
+shows "II (Tmap \<sigma> t)"
 using assms(1) proof induct 
-  case (G_I_intro B t)   note B = G_I_intro(1)  
-  have G: "G (\<lambda>t. I (Tmap \<sigma> t)) B t"
-  apply(rule G_mmono[OF _ G_I_intro(1,2)]) using \<sigma> by auto
-  have G: "G (\<lambda>t. I (Tmap \<sigma> (Tmap (inv \<sigma>) t))) (image \<sigma> B) (Tmap \<sigma> t)"
-  using G_eequiv[OF \<sigma> B G] . 
-  have "G I (image \<sigma> B) (Tmap \<sigma> t)" 
-  apply(rule G_mmono[OF _ _ G])
-    subgoal using \<sigma> 
-    by auto (metis Tmap_comp' Tmap_id id_apply ssbij_inv ssbij_invL)
-    subgoal using small_image[OF B] . .
-  thus ?case using small_image[OF B] by (subst I.simps, auto)
+  case (GG_II_intro xs t)   (* note xs = GG_II_intro(1) *) 
+  have GG: "GG (\<lambda>t. II (Tmap \<sigma> t)) xs t"
+  apply(rule GG_mmono[OF _ GG_II_intro(1)]) using \<sigma> by auto
+  have GG: "GG (\<lambda>t. II (Tmap \<sigma> (Tmap (inv \<sigma>) t))) (Bmap \<sigma> xs) (Tmap \<sigma> t)"
+  using GG_eequiv[OF \<sigma> GG] .
+  have "GG II (Bmap \<sigma> xs) (Tmap \<sigma> t)" 
+  apply(rule GG_mmono[OF _ GG])
+  using \<sigma> 
+  by auto (metis Tmap_comp' Tmap_id id_apply ssbij_inv ssbij_invL) 
+  thus ?case by (subst II.simps, auto)
 qed
 
-lemma G_small_mono'[mono]: "\<And>R R' B t.  R \<le> R' \<Longrightarrow> 
- small B \<and> B \<inter> Tfvars t = {} \<and> G R B t \<longrightarrow> small B \<and> B \<inter> Tfvars t = {} \<and> G R' B t"
-  using G_mmono by blast
+lemma GG_mmono'[mono]: "\<And>R R' xs t.  R \<le> R' \<Longrightarrow> 
+ Bvars xs \<inter> Tfvars t = {} \<and> GG R xs t \<longrightarrow> Bvars xs \<inter> Tfvars t = {} \<and> GG R' xs t"
+  using GG_mmono by blast
 
-inductive I' :: "'T \<Rightarrow> bool" where 
-G_I'_intro: "small B \<Longrightarrow> B \<inter> Tfvars t = {} \<Longrightarrow> G I' B t \<Longrightarrow> I' t"
+inductive II' :: "'T \<Rightarrow> bool" where 
+GG_II'_intro: "Bvars xs \<inter> Tfvars t = {} \<Longrightarrow> GG II' xs t \<Longrightarrow> II' t"
 
-lemma I'_imp_I: "I' t \<Longrightarrow> I t"
-apply(induct rule: I'.induct)
-by (smt (verit) G_mmono I.simps predicate1I) 
+lemma II'_imp_II: "II' t \<Longrightarrow> II t"
+apply(induct rule: II'.induct)
+by (smt (verit) GG_mmono II.simps predicate1I) 
 
-lemma I'_equiv: 
-assumes "I' t" and \<sigma>: "ssbij \<sigma>" "wfBij \<sigma>"
-shows "I' (Tmap \<sigma> t)"
+lemma II'_equiv: 
+assumes "II' t" and \<sigma>: "ssbij \<sigma>" "wfBij \<sigma>"
+shows "II' (Tmap \<sigma> t)"
 using assms(1) proof induct
-  case (G_I'_intro B t)  note B = G_I'_intro(1,2)   
-  have G: "G (\<lambda>t. I' (Tmap \<sigma> t)) B t"
-  apply(rule G_mmono[OF _ G_I'_intro(1,3)]) using \<sigma> by auto
-  have BB: "image \<sigma> B \<inter> Tfvars (Tmap \<sigma> t) = {}" using image_Tfvars_disj[OF \<sigma>(1) G_I'_intro(2)] .    
-  have G: "G (\<lambda>t. I' (Tmap \<sigma> (Tmap (inv \<sigma>) t))) (image \<sigma> B) (Tmap \<sigma> t)"
-  using G_eequiv[OF \<sigma> B(1) G] .
-  have 0: "(\<lambda>t. I' (Tmap \<sigma> (Tmap (inv \<sigma>) t))) = I'"
+  case (GG_II'_intro xs t)  note B = GG_II'_intro(1)   
+  have GG: "GG (\<lambda>t. II' (Tmap \<sigma> t)) xs t" 
+  apply(rule GG_mmono[OF _ GG_II'_intro(2)]) using \<sigma> by auto
+  have BB: "Bvars (Bmap \<sigma> xs) \<inter> Tfvars (Tmap \<sigma> t) = {}" using image_Tfvars_disj[OF \<sigma>(1) GG_II'_intro(1)] 
+  using Bmap_Bvars[OF \<sigma>(1)] by fastforce 
+  have GG: "GG (\<lambda>t. II' (Tmap \<sigma> (Tmap (inv \<sigma>) t))) (Bmap \<sigma> xs) (Tmap \<sigma> t)"
+  using GG_eequiv[OF \<sigma> GG] .
+  have 0: "(\<lambda>t. II' (Tmap \<sigma> (Tmap (inv \<sigma>) t))) = II'"
   unfolding fun_eq_iff  
   by (metis Tmap_comp' Tmap_cong_id \<sigma>(1) id_apply ssbij_comp ssbij_inv ssbij_invL)
-  have G: "G I' (image \<sigma> B) (Tmap \<sigma> t)"
-  using G unfolding 0 .
-  show ?case using BB G small_image[OF B(1)] by (subst I'.simps, auto) 
+  have GG: "GG II' (Bmap \<sigma> xs) (Tmap \<sigma> t)"
+  using GG unfolding 0 .
+  show ?case using BB GG small_image by (subst II'.simps, auto) 
 qed
 
 end (* context IInduct1 *)
 
 
-locale IInduct = IInduct1 dummy Tmap Tfvars G closed wfBij
+locale IInduct = IInduct1 dummy Tmap Tfvars Bmap Bvars wfB GG 
 for dummy :: 'A 
-and
-Tmap :: "('A \<Rightarrow> 'A) \<Rightarrow> 'T \<Rightarrow> 'T"
+and Tmap :: "('A \<Rightarrow> 'A) \<Rightarrow> 'T \<Rightarrow> 'T"
 and Tfvars :: "'T \<Rightarrow> 'A set"
-and 
-G :: "('T \<Rightarrow> bool) \<Rightarrow> 'A set \<Rightarrow> 'T \<Rightarrow> bool"
-and closed and wfBij 
+and Bmap :: "('A \<Rightarrow> 'A) \<Rightarrow> 'B \<Rightarrow> 'B"
+and Bvars :: "'B \<Rightarrow> 'A set"
+and wfB
+and GG :: "('T \<Rightarrow> bool) \<Rightarrow> 'B \<Rightarrow> 'T \<Rightarrow> bool"
 +
 assumes 
-G_rrefresh: 
-"\<And>R B t. (\<forall>t. R t \<longrightarrow> I t) \<Longrightarrow> 
-         (\<forall>\<sigma> t. ssbij \<sigma> \<and> wfBij \<sigma> \<and> R t \<longrightarrow> R (Tmap \<sigma> t)) \<Longrightarrow> small B \<Longrightarrow> G R B t \<Longrightarrow> 
-         \<exists>C. small C \<and> C \<inter> Tfvars t = {} \<and> G R C t"
+GG_rrefresh: 
+"\<And>R xs t. (\<forall>t. R t \<longrightarrow> II t) \<Longrightarrow> 
+         (\<forall>\<sigma> t. ssbij \<sigma> \<and> wfBij \<sigma> \<and> R t \<longrightarrow> R (Tmap \<sigma> t)) \<Longrightarrow> GG R xs t \<Longrightarrow> 
+         \<exists>ys. Bvars ys \<inter> Tfvars t = {} \<and> GG R ys t"
 
 
 context IInduct
 begin
 
-(* NB: The following could replace G_refresh in the axiomatization. 
-It has the advantage that it is weaker, but also two disadvantages:
--- it depends on the "auxiliary" defined predicate I'
--- the dependency on I' seems truly inessential, in that in concrete cases 
-all that one needs to use is the equivariance of I'
+(* NB: The following could replace GG_refresh in the axiomatization. 
+IIt has the advantage that it is weaker, but also two disadvantages:
+-- it depends on the "auxiliary" defined predicate II'
+-- the dependency on II' seems truly inessential, in that in concrete cases 
+all that one needs to use is the equivariance of II'
 Later note: in the end, if was useful for getting in inductive information, 
-namely strenthening G_refresh to further assume that R implies I ("\<forall>t. R t \<longrightarrow> I t").  
+namely strenthening GG_refresh to further assume that R implies II ("\<forall>t. R t \<longrightarrow> II t").  
  *)
-lemma G_refresh_I': 
-"\<And>B t. small B \<Longrightarrow> G I' B t \<Longrightarrow> \<exists>C. small C \<and> C \<inter> Tfvars t = {} \<and> G I' C t"
-using G_rrefresh I'_equiv by (simp add: I'_imp_I)
+lemma GG_refresh_II': 
+"\<And>xs t. GG II' xs t \<Longrightarrow> \<exists>ys. Bvars ys \<inter> Tfvars t = {} \<and> GG II' ys t"
+using GG_rrefresh II'_equiv by (simp add: II'_imp_II)
 
-lemma I_imp_I': "I t \<Longrightarrow> I' t"
-proof(induct rule: I.induct)
-  case (G_I_intro B t)
-  hence G: "G I' B t" by (metis (no_types, lifting) G_mmono predicate1I)
-  note sB = `small B` 
-  from G_refresh_I'[OF sB G]
-  obtain C where 0: "small C" "C \<inter> Tfvars t = {}" "G I' C t" by auto 
-  show ?case using I'.intros[OF 0] .
+lemma II_imp_II': "II t \<Longrightarrow> II' t"
+proof(induct rule: II.induct)
+  case (GG_II_intro xs t)
+  hence GG: "GG II' xs t" by (metis (no_types, lifting) GG_mmono predicate1I)
+  from GG_refresh_II'[OF GG]
+  obtain ys where 0: "Bvars ys \<inter> Tfvars t = {}" "GG II' ys t" by auto 
+  show ?case using II'.intros[OF 0] .
 qed
 
-lemma I_eq_I': "I = I'"
+lemma II_eq_II': "II = II'"
 apply(rule ext)
 subgoal for t
 apply(rule iffI)
-  subgoal using I_imp_I' by auto 
-  subgoal using I'_imp_I by auto . .
+  subgoal using II_imp_II' by auto 
+  subgoal using II'_imp_II by auto . .
  
 end (* context IInduct *)
 
 
 (* The locale with the more restricted rule, in the style of Urban-Berghofer-Norrish: *)
-locale IInduct_simple = IInduct1 dummy Tmap Tfvars G closed wfBij 
+locale IInduct_simple = IInduct1 dummy Tmap Tfvars Bmap Bvars wfB GG 
 for dummy :: 'A 
-and
-Tmap :: "('A \<Rightarrow> 'A) \<Rightarrow> 'T \<Rightarrow> 'T"
+and Tmap :: "('A \<Rightarrow> 'A) \<Rightarrow> 'T \<Rightarrow> 'T"
 and Tfvars :: "'T \<Rightarrow> 'A set"
-and 
-G :: "('T \<Rightarrow> bool) \<Rightarrow> 'A set \<Rightarrow> 'T \<Rightarrow> bool"
-and closed and wfBij 
+and Bmap :: "('A \<Rightarrow> 'A) \<Rightarrow> 'B \<Rightarrow> 'B"
+and Bvars :: "'B \<Rightarrow> 'A set"
+and wfB
+and GG :: "('T \<Rightarrow> bool) \<Rightarrow> 'B \<Rightarrow> 'T \<Rightarrow> bool"
 +
 assumes 
-G_ffresh: "\<And>R B t. small B \<Longrightarrow> G R B t \<Longrightarrow> B \<inter> Tfvars t = {}"
+GG_ffresh: "\<And>R xs t. GG R xs t \<Longrightarrow> Bvars xs \<inter> Tfvars t = {}"
+
 
 sublocale IInduct_simple < IInduct apply standard
-  subgoal using G_ffresh by blast . 
+  subgoal using GG_ffresh by blast . 
 
 
 context IInduct 
 begin 
   
 (* Barendregt-enhanced (strong) induction. 
-NB: we get freshness for t as well, as a bonus (even though the inductive definition of I 
+NB: we get freshness for t as well, as a bonus (even though the inductive definition of II 
 needs not guarantee that -- see again the case of beta-reduction)
  *)
 
 
-theorem BE_induct[consumes 2]: 
+theorem BE_iinduct[consumes 2]: 
 (* Parameters: *)
 fixes Pfvars :: "'P \<Rightarrow> 'A set"
 assumes small_Pfvars: "\<And>p. small (Pfvars p)" 
 (* *)
-assumes I: "I (t::'T)"
-and strong: "\<And> p B t. small B \<Longrightarrow> B \<inter> Pfvars p = {} \<Longrightarrow> B \<inter> Tfvars t = {} \<Longrightarrow> 
-      G (\<lambda>t'. I t' \<and> (\<forall>p'. R p' t')) B t \<Longrightarrow> R p t"
+assumes II: "II (t::'T)"
+and strong: "\<And> p xs t. Bvars xs \<inter> Pfvars p = {} \<Longrightarrow> Bvars xs \<inter> Tfvars t = {} \<Longrightarrow> 
+      GG (\<lambda>t'. II t' \<and> (\<forall>p'. R p' t')) xs t \<Longrightarrow> R p t"
 shows "R p t"
 proof- 
   {fix \<sigma> assume \<sigma>: "ssbij \<sigma>" "wfBij \<sigma>"
    have "R p (Tmap \<sigma> t)"
-   using I \<sigma> unfolding I_eq_I' proof(induct arbitrary: \<sigma> p)
-     fix B t \<sigma> p  
-     assume small_B: "small B" and vt: "B \<inter> Tfvars t = {}" (* this additional vt assumption is what we have gained 
-     by transitioning from I to I', whose inductive definition has this freshness side-condition *)
-     and G: "G (\<lambda>t'. I' t' \<and> (\<forall>\<sigma>'. ssbij \<sigma>' \<longrightarrow> wfBij \<sigma>' \<longrightarrow> (\<forall>p'. R p' (Tmap \<sigma>' t')))) B t" and \<sigma>: "ssbij \<sigma>" "wfBij \<sigma>"
+   using II \<sigma> unfolding II_eq_II' proof(induct arbitrary: \<sigma> p)
+     fix xs t \<sigma> p  
+     assume vt: "Bvars xs \<inter> Tfvars t = {}" (* this additional vt assumption is what we have gained 
+     by transitioning from II to II', whose inductive definition has this freshness side-condition *)
+     and GG: "GG (\<lambda>t'. II' t' \<and> (\<forall>\<sigma>'. ssbij \<sigma>' \<longrightarrow> wfBij \<sigma>' \<longrightarrow> (\<forall>p'. R p' (Tmap \<sigma>' t')))) xs t" 
+     and \<sigma>: "ssbij \<sigma>" "wfBij \<sigma>"
 
-     (* have "I' t"  
-       by (metis (no_types, lifting) G I.simps I_eq_I' IInduct1.G_mono IInduct1_axioms predicate1I small_B)
-     hence I_T: "I t" using I'_imp_I by auto
-     hence "I (Tmap \<sigma> t)" by (simp add: I_equiv \<sigma>(1) \<sigma>(2)) *)
+     (* have "II' t"  
+       by (metis (no_types, lifting) GG II.simps II_eq_II' IInduct1.GG_mmono IInduct1_axioms predicate1II small_B)
+     hence II_T: "II t" using II'_imp_II by auto
+     hence "II (Tmap \<sigma> t)" by (simp add: II_equiv \<sigma>(1) \<sigma>(2)) *)
 
-     define B' where B': "B' \<equiv> \<sigma> ` B"
-     have small_B': "small B'"  
-       using B' small_B small_image by blast
+     define xs' where xs': "xs' \<equiv> Bmap \<sigma> xs"
 
-     have "closed B" using G_closed[OF G] .
-     hence clB': "closed B'"  
-     unfolding B' using closed_wfBij[OF \<sigma>(1,2)] by simp
 
-     have v't: "B' \<inter> Tfvars (Tmap \<sigma> t) = {}" 
-     using vt unfolding B'  
-     using image_Tfvars_disj \<sigma> by blast 
+     have "wfB xs" using GG_wfB[OF GG] .
+     hence wfB': "wfB xs'"  
+     unfolding xs' using \<sigma>(2) wfBij_def by auto 
+
+     have v't: "Bvars xs' \<inter> Tfvars (Tmap \<sigma> t) = {}" 
+     using vt unfolding xs'  
+     using image_Tfvars_disj \<sigma>  
+     by (meson Bmap_Bvars Int_subset_empty1)
 
      have small_p_t: "small (Pfvars p \<union> Tfvars (Tmap \<sigma> t))"  
        by (simp add: small_Pfvars small_Tfvars small_Un)
 
-     obtain \<rho> where \<rho>: "ssbij \<rho>" "wfBij \<rho>" "\<rho> ` B' \<inter> (Pfvars p \<union> Tfvars (Tmap \<sigma> t)) = {}" "\<forall>a \<in> Tfvars (Tmap \<sigma> t). \<rho> a = a"
-     using small_ssbij_closed[of B' "Pfvars p \<union> Tfvars (Tmap \<sigma> t)" "Tfvars (Tmap \<sigma> t)"] 
-     using small_Tfvars small_B' small_p_t v't clB' by metis
+     obtain \<rho> where \<rho>: "ssbij \<rho>" "wfBij \<rho>" "\<rho> ` (Bvars xs') \<inter> (Pfvars p \<union> Tfvars (Tmap \<sigma> t)) = {}" 
+     "\<forall>a \<in> Tfvars (Tmap \<sigma> t). \<rho> a = a"
+     (* using extend_wfBij[of B' "Pfvars p \<union> Tfvars (Tmap \<sigma> t)" "Tfvars (Tmap \<sigma> t)"] 
+     using small_Tfvars small_B' small_p_t v't clB' by metis *) sorry
  
-     have fresh_p: "image \<rho> B' \<inter> Pfvars p = {}" 
-     and fresh_t: "image \<rho> B' \<inter> Tfvars (Tmap \<sigma> t) = {}"  
+     have "\<rho> ` (Bvars xs') \<inter> Pfvars p = {}" 
+     and "\<rho> ` (Bvars xs') \<inter> Tfvars (Tmap \<sigma> t) = {}"  
      using \<rho>(1,2,3) by auto
+     hence fresh_p: "Bvars (Bmap \<rho> xs') \<inter> Pfvars p = {}" 
+     and fresh_t: "Bvars (Bmap \<rho> xs') \<inter> Tfvars (Tmap \<sigma> t) = {}"
+     using \<rho>(1) Bmap_Bvars by fastforce+ 
 
      hence "Tmap \<rho> (Tmap \<sigma> t) = Tmap \<sigma> t" 
      using Tmap_cong_id[OF \<rho>(1,4)] by blast
@@ -372,42 +411,63 @@ proof-
      have 1[simp]: "\<sigma>'' \<circ> inv (\<rho> o \<sigma>) = id" 
      unfolding \<sigma>'' using \<rho>\<sigma> ssbij_invL by auto  
    
-     have "G (\<lambda>t'. I' t' \<and> (\<forall>p'. R p' (Tmap \<sigma>'' t'))) B t"  
-     apply(rule G_mmono[OF _ small_B G]) using ss_\<sigma>'' by auto
-     hence G: "G (\<lambda>t'. I' (Tmap \<sigma>'' t') \<and> (\<forall>p'. R p' (Tmap \<sigma>'' t'))) B t" 
-     using I'_equiv[OF _ ss_\<sigma>'']  
-     by (smt (verit, del_insts) G_mmono predicate1I small_B) 
-     have G: "G (\<lambda>t'. I' (Tmap \<sigma>'' (Tmap (inv (\<rho> o \<sigma>)) t')) \<and> (\<forall>p'. R p' (Tmap \<sigma>'' (Tmap (inv (\<rho> o \<sigma>)) t')))) 
-                (image (\<rho> o \<sigma>) B) (Tmap (\<rho> o \<sigma>) t) " 
-     using G_eequiv[OF \<rho>\<sigma> small_B G] .
+     have "GG (\<lambda>t'. II' t' \<and> (\<forall>p'. R p' (Tmap \<sigma>'' t'))) xs t"  
+     apply(rule GG_mmono[OF _ GG]) using ss_\<sigma>'' by auto
+     hence GG: "GG (\<lambda>t'. II' (Tmap \<sigma>'' t') \<and> (\<forall>p'. R p' (Tmap \<sigma>'' t'))) xs t" 
+     using II'_equiv[OF _ ss_\<sigma>'']  
+     by (smt (verit, del_insts) GG_mmono predicate1I) 
+     have GG: "GG (\<lambda>t'. II' (Tmap \<sigma>'' (Tmap (inv (\<rho> o \<sigma>)) t')) \<and> 
+                      (\<forall>p'. R p' (Tmap \<sigma>'' (Tmap (inv (\<rho> o \<sigma>)) t')))) 
+                 (Bmap (\<rho> o \<sigma>) xs) 
+                 (Tmap (\<rho> o \<sigma>) t) " 
+     using GG_eequiv[OF \<rho>\<sigma> GG] .
      
-     have G: "G (\<lambda>t'. I' (Tmap (\<sigma>'' o inv (\<rho> o \<sigma>)) t') \<and> (\<forall>p'. R p' (Tmap (\<sigma>'' o inv (\<rho> o \<sigma>)) t'))) 
-                (image \<rho> B') (Tmap \<sigma> t) "  
-     unfolding B' unfolding image_comp 0[symmetric]
-     apply(rule G_mmono[OF _ _ G])
-       subgoal by auto (metis "1" Tmap_comp' \<rho>\<sigma> ss_\<sigma>'' ssbij_inv)+
-       subgoal by (simp add: small_B small_image) .
+     have GG: "GG (\<lambda>t'. II' (Tmap (\<sigma>'' o inv (\<rho> o \<sigma>)) t') \<and> (\<forall>p'. R p' (Tmap (\<sigma>'' o inv (\<rho> o \<sigma>)) t'))) 
+                (Bmap \<rho> xs') (Tmap \<sigma> t) "  
+     unfolding xs' unfolding image_comp 0[symmetric] Bmap_comp'[symmetric, OF \<rho>(1) \<sigma>(1)] 
+     apply(rule GG_mmono[OF _ GG])
+     by auto (metis 1 Tmap_comp' Tmap_id \<sigma>'' id_apply ss_\<sigma>''(1) ssbij_inv)+    
 
-     have G: "G (\<lambda>t'. I' t' \<and> (\<forall>p'. R p' t')) (image \<rho> B') (Tmap \<sigma> t)" 
-     apply(rule G_mmono[OF _ _ G]) 
-       subgoal by (simp add: Tmap_id)
-       subgoal using small_image[OF small_B'] . .
-
-     note sm = small_image[OF small_B']
+     have GG: "GG (\<lambda>t'. II' t' \<and> (\<forall>p'. R p' t')) (Bmap \<rho> xs') (Tmap \<sigma> t)" 
+     apply(rule GG_mmono[OF _ GG]) 
+     by auto
 
      show "R p (Tmap \<sigma> t)" 
-     using strong[OF sm fresh_p fresh_t G[unfolded I_eq_I'[symmetric]]] .
+     using strong[OF fresh_p fresh_t GG[unfolded II_eq_II'[symmetric]]] .
   qed
   }
   from this[of id] show ?thesis 
-  by (simp add: Tmap_id ssbij_id)
+  by (simp add: ssbij_id)
 qed
 
 end (* context IInduct *)
 
 
 
-(* VERSIONS OF THE LOCALES WITHOUT wfBij AND closed, which work in 99% of the cases: *)
+(* VERSIONS OF THE LOCALES WITH SMALL SETS INSTEAD OF BINDER-LIKE ENTITIES, which work in 99% of the cases: *)
+
+locale Components = Small dummy
+for dummy :: 'A
++
+fixes (* 'T: term-like entities *)
+Tmap :: "('A \<Rightarrow> 'A) \<Rightarrow> 'T \<Rightarrow> 'T"
+and Tfvars :: "'T \<Rightarrow> 'A set"
+assumes  
+Tmap_id: "Tmap id = id"
+and
+Tmap_comp: "\<And>\<sigma> \<tau>. ssbij \<sigma> \<Longrightarrow> ssbij \<tau> \<Longrightarrow> Tmap (\<sigma> o \<tau>) = Tmap \<sigma> o Tmap \<tau>"
+and
+small_Tfvars: "\<And>t. small (Tfvars t)"
+and 
+Tmap_Tfvars: "\<And>t \<sigma>. ssbij \<sigma> \<Longrightarrow> Tfvars (Tmap \<sigma> t) \<subseteq> \<sigma> ` (Tfvars t)"
+and
+Tmap_cong_id: "\<And>t \<sigma>. ssbij \<sigma> \<Longrightarrow> (\<forall>a\<in>Tfvars t. \<sigma> a = a) \<Longrightarrow> Tmap \<sigma> t = t"
+
+sublocale Components < CComponents where Tmap = Tmap and Tfvars = Tfvars and 
+Bmap = image and Bvars = id and wfB = small apply standard 
+using Tmap_id Tmap_comp small_Tfvars Tmap_Tfvars Tmap_cong_id apply auto
+by fastforce
+
 
 locale Induct1 = Components dummy Tmap Tfvars 
 for dummy :: 'A 
@@ -421,10 +481,69 @@ assumes
 G_mono: "\<And>R R' B t. R \<le> R' \<Longrightarrow> small B \<Longrightarrow> G R B t \<Longrightarrow> G R' B t"
 and 
 G_equiv: "\<And>\<sigma> R B t. ssbij \<sigma> \<Longrightarrow> small B \<Longrightarrow> G R B t \<Longrightarrow> G (\<lambda>t'. R (Tmap (inv \<sigma>) t')) (image \<sigma> B) (Tmap \<sigma> t)"
+begin 
+
+definition GG where "GG R B t \<equiv> small B \<and> G R B t"
+
+lemma GG_mmono: "R \<le> R' \<Longrightarrow> GG R B t \<Longrightarrow> GG R' B t"
+by (simp add: GG_def G_mono)
+
+lemma GG_eequiv: "ssbij \<sigma> \<Longrightarrow> wfBij \<sigma> \<Longrightarrow> 
+   GG R B t \<Longrightarrow> GG (\<lambda>t'. R (Tmap (inv \<sigma>) t')) (\<sigma> ` B) (Tmap \<sigma> t)"
+using GG_def G_equiv small_image by force
+
+lemma GG_wfB: "GG R B t \<Longrightarrow> small B"
+unfolding GG_def by auto
+
+lemma extend_wfBij: 
+"\<And>A. small A \<Longrightarrow> bsmall A \<Longrightarrow> bij_betw \<rho> A B \<Longrightarrow> wfBij \<rho> \<Longrightarrow> 
+     \<exists>\<rho>'. ssbij \<rho>' \<and> wfBij \<rho>' \<and> (\<forall>a\<in>A. \<rho>' a = \<rho> a)"
+unfolding wfBij_def sorry
+
+end (* context Induct1 *)
+
+sublocale Induct1 < IInduct1 where Tmap = Tmap and Tfvars = Tfvars and 
+Bmap = image and Bvars = id and wfB = small and GG = GG apply standard 
+using GG_mmono GG_eequiv GG_wfB extend_wfBij by auto
+
+context Induct1
+begin 
+
+
+lemma G_mono'[mono]: "\<And>R R' B t. R \<le> R' \<Longrightarrow> small B \<and> G R B t \<longrightarrow> small B \<and> G R' B t"
+using G_mono by auto
+
+
+inductive I :: "'T \<Rightarrow> bool" where 
+G_I_intro: "small B \<Longrightarrow> G I B t \<Longrightarrow> I t"
+
+lemma "I \<equiv> lfp (\<lambda>R t. \<exists>B. small B \<and> G R B t)"
+using I_def[simplified] .
+
+lemma I_eq_II: "I = II"
+apply(intro ext, rule iffI)
+  subgoal for t apply (induct rule: I.induct)
+    subgoal for B t apply(rule II.intros[of B t])
+    unfolding GG_def 
+    by (metis (no_types, lifting) G_mono predicate1I) .
+  subgoal for t apply (induct rule: II.induct)
+    subgoal for B t apply(rule I.intros[of B t])
+    unfolding GG_def 
+    by (simp,metis (no_types, lifting) G_mono predicate1I) . .
  
-sublocale Induct1 < IInduct1 where Tmap = Tmap and Tfvars = Tfvars and G = G 
-and closed = "\<lambda>_. True" and wfBij = "\<lambda>_. True" apply standard
-using G_mono G_equiv small_ssbij by auto
+lemma I_equiv: 
+assumes "I t" and \<sigma>: "ssbij \<sigma>" "wfBij \<sigma>"
+shows "I (Tmap \<sigma> t)"
+using II_equiv I_eq_II assms by auto
+
+
+lemma ssbij_wfBij: "ssbij \<sigma> \<Longrightarrow> wfBij \<sigma>"
+unfolding wfBij_def ssbij_def 
+using bij_card_of_ordIso ordIso_ordLess_trans ordIso_symmetric small_def by blast
+
+end (* context Induct1 *)
+ 
+
 
 locale Induct = Induct1 dummy Tmap Tfvars G  
 for dummy :: 'A 
@@ -439,7 +558,41 @@ G_refresh:
 "\<And>R B t. (\<forall>t. R t \<longrightarrow> I t) \<Longrightarrow> 
          (\<forall>\<sigma> t. ssbij \<sigma> \<and> R t \<longrightarrow> R (Tmap \<sigma> t)) \<Longrightarrow> small B \<Longrightarrow> G R B t \<Longrightarrow> 
          \<exists>C. small C \<and> C \<inter> Tfvars t = {} \<and> G R C t"
+begin
 
+lemma GG_rrefresh: 
+assumes "\<forall>t. R t \<longrightarrow> II t" "\<forall>\<sigma> t. ssbij \<sigma> \<and> wfBij \<sigma> \<and> R t \<longrightarrow> R (Tmap \<sigma> t)" "GG R B t"
+shows "\<exists>C. C \<inter> Tfvars t = {} \<and> GG R C t"
+using G_refresh[OF assms(1)[unfolded I_eq_II[symmetric]]]
+using G_refresh[of R B t] unfolding GG_def I_eq_II[symmetric] 
+by (metis GG_def assms(2) assms(3) ssbij_wfBij)
+
+end (* context Induct *)
+
+sublocale Induct < IInduct where Tmap = Tmap and Tfvars = Tfvars and 
+Bmap = image and Bvars = id and wfB = small and GG = GG apply standard 
+by (simp add: GG_rrefresh)
+
+
+context Induct
+begin
+thm BE_iinduct 
+
+theorem BE_induct[consumes 2]: 
+(* Parameters: *)
+fixes Pfvars :: "'P \<Rightarrow> 'A set"
+assumes small_Pfvars: "\<And>p. small (Pfvars p)" 
+(* *)
+assumes I: "I (t::'T)"
+and strong: "\<And> p B t. small B \<Longrightarrow> B \<inter> Pfvars p = {} \<Longrightarrow> B \<inter> Tfvars t = {} \<Longrightarrow> 
+      G (\<lambda>t'. I t' \<and> (\<forall>p'. R p' t')) B t \<Longrightarrow> R p t"
+shows "R p t"
+apply(rule BE_iinduct[of Pfvars _ R p, OF small_Pfvars I[unfolded I_eq_II]])
+subgoal for p B t apply(rule strong[of B p t]) 
+by (auto simp add: GG_def I_eq_II) .
+
+
+end (* context Induct *)
 
 (* The locale with the more restricted rule, in the style of Urban-Berghofer-Norrish: *)
 locale Induct_simple = Induct1 dummy Tmap Tfvars G 
@@ -454,16 +607,10 @@ assumes
 G_fresh: "\<And>R B t. small B \<Longrightarrow> G R B t \<Longrightarrow> B \<inter> Tfvars t = {}"
 
 
-sublocale Induct < IInduct where Tmap = Tmap and Tfvars = Tfvars and G = G 
-and closed = "\<lambda>_. True" and wfBij = "\<lambda>_. True" apply standard using G_refresh by auto
 
 
-context Induct
-begin
-thm BE_induct 
-end 
 
- 
+
 
 
 end 
